thys/Pairing_Heap/Pairing_Heap_List2.thy
@@ -15,14 +15,19 @@ datatype 'a hp = Hp 'a (hps: "'a hp list")
 
 type_synonym 'a heap = "'a hp option"
 
-fun get_min  :: "'a :: linorder heap \<Rightarrow> 'a" where
+hide_const (open) insert
+
+fun get_min  :: "'a heap \<Rightarrow> 'a" where
 "get_min (Some(Hp x _)) = x"
 
-fun link :: "'a :: linorder hp \<Rightarrow> 'a hp \<Rightarrow> 'a hp" where
+context linorder
+begin
+
+fun link :: "'a hp \<Rightarrow> 'a hp \<Rightarrow> 'a hp" where
 "link (Hp x lx) (Hp y ly) = 
     (if x < y then Hp x (Hp y ly # lx) else Hp y (Hp x lx # ly))"
 
-fun merge :: "'a :: linorder heap \<Rightarrow> 'a heap \<Rightarrow> 'a heap" where
+fun merge :: "'a heap \<Rightarrow> 'a heap \<Rightarrow> 'a heap" where
 "merge h None = h" |
 "merge None h = h" |
 "merge (Some h1) (Some h2) = Some(link h1 h2)"
@@ -30,50 +35,54 @@ fun merge :: "'a :: linorder heap \<Rightarrow> 'a heap \<Rightarrow> 'a heap" w
 lemma merge_None[simp]: "merge None h = h"
 by(cases h)auto
 
-hide_const (open) insert
-
-fun insert :: "'a \<Rightarrow> 'a :: linorder heap \<Rightarrow> 'a heap" where
+fun insert :: "'a \<Rightarrow> 'a heap \<Rightarrow> 'a heap" where
 "insert x None = Some(Hp x [])" |
 "insert x (Some h) = Some(link (Hp x []) h)"
 
-fun pass\<^sub>1 :: "'a :: linorder hp list \<Rightarrow> 'a hp list" where
+fun pass\<^sub>1 :: "'a hp list \<Rightarrow> 'a hp list" where
   "pass\<^sub>1 [] = []"
 | "pass\<^sub>1 [h] = [h]" 
 | "pass\<^sub>1 (h1#h2#hs) = link h1 h2 # pass\<^sub>1 hs"
 
-fun pass\<^sub>2 :: "'a :: linorder hp list \<Rightarrow> 'a heap" where
+fun pass\<^sub>2 :: "'a hp list \<Rightarrow> 'a heap" where
   "pass\<^sub>2 [] = None"
 | "pass\<^sub>2 (h#hs) = Some(case pass\<^sub>2 hs of None \<Rightarrow> h | Some h' \<Rightarrow> link h h')"
 
-fun mergepairs :: "'a :: linorder hp list \<Rightarrow> 'a heap" where
-  "mergepairs [] = None"
-| "mergepairs [h] = Some h" 
-| "mergepairs (h1 # h2 # hs) =
-  Some(let h12 = link h1 h2 in case mergepairs hs of None \<Rightarrow> h12 | Some h \<Rightarrow> link h12 h)"
+fun merge_pairs :: "'a hp list \<Rightarrow> 'a heap" where
+  "merge_pairs [] = None"
+| "merge_pairs [h] = Some h" 
+| "merge_pairs (h1 # h2 # hs) =
+  Some(let h12 = link h1 h2 in case merge_pairs hs of None \<Rightarrow> h12 | Some h \<Rightarrow> link h12 h)"
 
-fun del_min :: "'a :: linorder heap \<Rightarrow> 'a heap" where
+fun del_min :: "'a heap \<Rightarrow> 'a heap" where
   "del_min None = None"
 | "del_min (Some(Hp x hs)) = pass\<^sub>2 (pass\<^sub>1 hs)"
+
+end (* linorder *)
 
 
 subsection \<open>Correctness Proofs\<close>
 
 text \<open>An optimization:\<close>
 
-lemma mergepairs_pass12: "mergepairs hs = pass\<^sub>2 (pass\<^sub>1 hs)"
-by (induction hs rule: mergepairs.induct) (auto split: option.split)
+lemma pass12_merge_pairs: "pass\<^sub>2 (pass\<^sub>1 hs) = merge_pairs hs"
+by (induction hs rule: merge_pairs.induct) (auto split: option.split)
 
-declare mergepairs_pass12[symmetric, code_unfold]
+declare pass12_merge_pairs[code_unfold]
 
 
 subsubsection \<open>Invariants\<close>
 
-fun php :: "'a :: linorder hp \<Rightarrow> bool" where
+context linorder
+begin
+
+fun php :: "'a hp \<Rightarrow> bool" where
 "php (Hp x hs) = (\<forall>h \<in> set hs. (\<forall>y \<in> set_hp h. x \<le> y) \<and> php h)"
 
-definition invar :: "'a :: linorder heap \<Rightarrow> bool" where
+definition invar :: "'a heap \<Rightarrow> bool" where
 "invar ho = (case ho of None \<Rightarrow> True | Some h \<Rightarrow> php h)"
 
+end
 
 lemma php_link: "php h1 \<Longrightarrow> php h2 \<Longrightarrow> php (link h1 h2)"
 by (induction h1 h2 rule: link.induct) fastforce+
@@ -128,16 +137,13 @@ by (induction h1 h2 rule: merge.induct)
 lemma mset_insert: "mset_heap (insert a h) = {#a#} + mset_heap h"
 by(cases h) (auto simp add: mset_link mset_heap_def insert_def)
 
-lemma mset_pass1:
-  "Union_mset(image_mset mset_hp (mset (pass\<^sub>1 hs))) = Union_mset(image_mset mset_hp (mset hs))"
-by(induction hs rule: pass\<^sub>1.induct)(auto simp: mset_link add_ac)
-
-lemma mset_pass2: "mset_heap (pass\<^sub>2 hs) = Union_mset(image_mset mset_hp(mset hs))"
-by(induction hs)(auto simp: mset_link mset_heap_def add_ac split: option.splits)
+lemma mset_merge_pairs: "mset_heap (merge_pairs hs) = Union_mset(image_mset mset_hp (mset hs))"
+by(induction hs rule: merge_pairs.induct)
+  (auto simp: mset_merge mset_link mset_heap_def Let_def split: option.split)
 
 lemma mset_del_min: "h \<noteq> None \<Longrightarrow>
   mset_heap (del_min h) = mset_heap h - {#get_min h#}"
 by(induction h rule: del_min.induct)
-  (auto simp: mset_heap_Some mset_pass1 mset_pass2)
+  (auto simp: mset_heap_Some pass12_merge_pairs mset_merge_pairs)
 
 end
